refactor: SubOperation follow AddOperation style

SP1Operations/SubOperation.lean
@@ -1,50 +1,66 @@
 import SP1Foundations
 
-@[reducible] def SubOperation (T : Type) := Word T
+structure SubOperation where
+  value : Word U16
 
 namespace SubOperation
 
 /-- `SubOperation` should result in wrapping addition of the outputs.
 Note that we ignore `is_real` for now. -/
-def spec (cols : SubOperation BabyBear) (a b : Word BabyBear) : Prop :=
-  a.isUInt32 → b.isUInt32 →
-    a.toNat = (cols.toNat + b.toNat) % 2^32
+def spec (cols : SubOperation) (a b : Word U16) (is_real : U2) : Prop :=
+  is_real = U2.one → a.toFin32_U16 - b.toFin32_U16 = cols.value.toFin32_U16
 
 /-- Constraints on `SubOperation` as extracted from the source code:
 Asserting expr 3: `(is_real * (is_real - 1))`
 Asserting expr 17: `(is_real * (((((((a[0] + 65536) - 1) - b[0]) - cols.value[0]) + 1) * 2013235201) * (((((((a[0] + 65536) - 1) - b[0]) - cols.value[0]) + 1) * 2013235201) - 1)))`
 Asserting expr 29: `(is_real * (((((((a[1] + 65536) - 1) - b[1]) - cols.value[1]) + ((((((a[0] + 65536) - 1) - b[0]) - cols.value[0]) + 1) * 2013235201)) * 2013235201) * (((((((a[1] + 65536) - 1) - b[1]) - cols.value[1]) + ((((((a[0] + 65536) - 1) - b[0]) - cols.value[0]) + 1) * 2013235201)) * 2013235201) - 1)))` -/
-def extractedConstraints (cols : SubOperation BabyBear)
-    (a b : Word BabyBear) (is_real : BabyBear) : List SP1Constraint :=
+def extractedConstraints (cols : SubOperation)
+    (a b : Word U16) (is_real : U2) : List SP1Constraint :=
   [
-  .assertZero (is_real * (is_real - 1)),
-  .assertZero (is_real * (((((((a[0] + 65536) - 1) - b[0]) - cols[0]) + 1) * 2013235201) * (((((((a[0] + 65536) - 1) - b[0]) - cols[0]) + 1) * 2013235201) - 1))),
-  .assertZero (is_real * (((((((a[1] + 65536) - 1) - b[1]) - cols[1]) + ((((((a[0] + 65536) - 1) - b[0]) - cols[0]) + 1) * 2013235201)) * 2013235201) * (((((((a[1] + 65536) - 1) - b[1]) - cols[1]) + ((((((a[0] + 65536) - 1) - b[0]) - cols[0]) + 1) * 2013235201)) * 2013235201) - 1))),
+  .assertZero (is_real.val * (((((((a[0] + (65536 : BabyBear)) - (1 : BabyBear)) - b[0]) - cols.value[0]) + 1) * (2013235201 : BabyBear)) * (((((((a[0] + (65536 : BabyBear)) - (1 : BabyBear)) - b[0]) - cols.value[0]) + 1) * (2013235201 : BabyBear)) - (1 : BabyBear)))),
+  .assertZero (is_real.val * (((((((a[1] + (65536 : BabyBear)) - (1 : BabyBear)) - b[1]) - cols.value[1]) + ((((((a[0] + (65536 : BabyBear)) - (1 : BabyBear)) - b[0]) - cols.value[0]) + 1) * (2013235201 : BabyBear))) * (2013235201 : BabyBear)) * (((((((a[1] + (65536 : BabyBear)) - (1 : BabyBear)) - b[1]) - cols.value[1]) + ((((((a[0] + (65536 : BabyBear)) - (1 : BabyBear)) - b[0]) - cols.value[0]) + 1) * (2013235201 : BabyBear))) * (2013235201 : BabyBear)) - (1 : BabyBear)))),
   ]
 
 /-- Cleaned up representation of the `SubOperation` constraints. -/
-def idealizedConstraints (cols : SubOperation BabyBear)
-    (a b : Word BabyBear) : Prop :=
+def idealizedConstraints (cols : SubOperation)
+    (a b : Word U16) (is_real : U2) : Prop :=
   let carry0 : BabyBear := 1
-  let carry1 : BabyBear := (a[0] + base - 1 - b[0] - cols[0] + carry0) * baseInv
-  let carry2 : BabyBear := (a[1] + base - 1 - b[1] - cols[1] + carry1) * baseInv
-  carry1 * (carry1 - 1) = 0 ∧ -- isBool check
-  carry2 * (carry2 - 1) = 0 -- isBool check
+  let carry1 : BabyBear := (a[0] + base - (1 : BabyBear) - b[0] - cols.value[0] + carry0) * baseInv
+  let carry2 : BabyBear := (a[1] + base - (1 : BabyBear) - b[1] - cols.value[1] + carry1) * baseInv
+  (is_real.val * carry1 * (carry1 - 1)) = 0 ∧ -- isBool check
+  (is_real.val * carry2 * (carry2 - 1)) = 0 -- isBool check
 
 /-- The idealized constraints are logically equivalent to the extracted ones when `is_real := 1` -/
 lemma extractedConstraints_iff_idealizedConstraints
-    (cols : SubOperation BabyBear) (a b : Word BabyBear) :
-    constraintList_toProp (cols.extractedConstraints a b 1) ↔ cols.idealizedConstraints a b := by
-  simp [extractedConstraints, idealizedConstraints]
+    (cols : SubOperation) (a b : Word U16) (is_real : U2) :
+    constraintList_toProp (cols.extractedConstraints a b is_real) ↔ cols.idealizedConstraints a b is_real := by
+  simp [extractedConstraints, idealizedConstraints, base, baseInv]
+  aesop
 
 /-- The extracted constraints on `SubOperation` imply the spec. -/
-theorem correct [Fact (Nat.Prime p)] (cols : SubOperation BabyBear)
-    (a b : Word BabyBear) (hcols : cols.isUInt32) :
-    cols.idealizedConstraints a b → cols.spec a b := by
+theorem correct [Fact (Nat.Prime p)] (cols : SubOperation)
+    (a b : Word U16) (is_real : U2) :
+    cols.idealizedConstraints a b is_real → cols.spec a b is_real := by
   -- Unfold the definitions of constraints and spec
   simp [idealizedConstraints, spec, sub_eq_zero, mul_eq_zero]
   -- Introduce all of the hypothesis from the constraints
-  intros h1 h2 ha_u32 hb_u32
+  intros h1 h2
+  -- Eliminate `is_real`
+  intro h_is_real
+  have is_real_val_eq_one : is_real.val = 1 := by aesop
+  rw [is_real_val_eq_one] at h1 h2
+  simp at h1 h2
+
+  simp [Word.toFin32_U16]
+
+  -- Extract the range constraint in U16
+  let _ : a[0].val.val < 65536 := a[0].in_range
+  let _ : b[0].val.val < 65536 := b[0].in_range
+  let _ : a[1].val.val < 65536 := a[1].in_range
+  let _ : b[1].val.val < 65536 := b[1].in_range
+  let _ : cols.value[0].val.val < 65536 := cols.value[0].in_range
+  let _ : cols.value[1].val.val < 65536 := cols.value[1].in_range
+
   -- Split on whether the lower limb addition causes a carry
   cases h1 with | inl h1 => ?_ | inr h1 => ?_
   all_goals -- In both cases can now reduce down to the `omega` linear constraint solver
